theories/MetaTheory/Typing.v
@@ -7,7 +7,7 @@ From Metaprog Require Import Data.Context MetaTheory.Conversion.
 (** * Basic definitions. *)
 (***********************************************************************)
 
-Definition is_TApp {s} (t : term s) : bool :=
+(*Definition is_TApp {s} (t : term s) : bool :=
   match t with
   | TApp _ _ => true
   | _ => false
@@ -17,9 +17,9 @@ Lemma is_TApp_rename {s s'} (ρ : ren s s') t :
   is_TApp (rename ρ t) = is_TApp t.
 Proof.
 induction t using term_ind' in s', ρ |- * ; simpl_subst ; cbn ; auto.
-Qed.
+Qed.*)
 
-(** [All_context P Γ] means that [P Γ' ty] holds on every type [Γ' |- ty]
+(** [All_context P Γ] means that [P Γ' ty] holds on every type [Γ' ⊢ ty]
     in the context [Γ]. *)
 Inductive All_context {s} (P : forall s', context s s' -> term s' -> Prop) :
   forall {s'}, context s s' -> Prop :=
@@ -39,7 +39,7 @@ Section All_spine.
 
   | All_spine_cons f_ty x a b arg args T :
       P s Σ Γ (TProd x a b) TType ->
-      Σ |- f_ty ≡ TProd x a b ->
+      Σ ⊢ f_ty ≡ TProd x a b ->
       All_spine Σ Γ (b[x := arg]) args T ->
       All_spine Σ Γ f_ty (arg :: args) T.
 End All_spine.
@@ -48,7 +48,7 @@ End All_spine.
 (** * Typing relation. *)
 (***********************************************************************)
 
-Reserved Notation "Σ ;; Γ |- t : T"
+Reserved Notation "Σ ;; Γ ⊢ t : T"
   (at level 50, no associativity, Γ at next level, t at next level, T at next level).
 
 Reserved Notation "'typing_context' Σ Γ"
@@ -56,62 +56,68 @@ Reserved Notation "'typing_context' Σ Γ"
 
 Unset Elimination Schemes.
 
-(** [Σ ;; Γ |- t : T] means that [t] has type [T] under context [Γ] in evar-map [Σ]. *)
+(** [Σ ;; Γ ⊢ t : T] means that [t] has type [T] under context [Γ] in evar-map [Σ]. *)
 Inductive typing {s} (Σ : evar_map) (Γ : context ∅ s) : term s -> term s -> Prop :=
 
 | typing_type :
     (*typing_context Σ Γ ->*)
-    Σ ;; Γ |- TType : TType
+    Σ ;; Γ ⊢ TType : TType
 
 | typing_var i ty :
     (*typing_context Σ Γ ->*)
     lookup_context i Γ = ty ->
-    Σ ;; Γ |- TVar i : ty
+    Σ ;; Γ ⊢ TVar i : ty
 
 | typing_lam x ty body body_ty :
-    Σ ;; Γ |- ty : TType ->
-    Σ ;; CCons Γ x ty |- body : body_ty ->
-    Σ ;; Γ |- TLam x ty body : TProd x ty body_ty
+    Σ ;; Γ ⊢ ty : TType ->
+    Σ ;; CCons Γ x ty ⊢ body : body_ty ->
+    Σ ;; Γ ⊢ TLam x ty body : TProd x ty body_ty
 
 | typing_prod x a b :
-    Σ ;; Γ |- a : TType ->
-    Σ ;; CCons Γ x a |- b : TType ->
-    Σ ;; Γ |- TProd x a b : TType
+    Σ ;; Γ ⊢ a : TType ->
+    Σ ;; CCons Γ x a ⊢ b : TType ->
+    Σ ;; Γ ⊢ TProd x a b : TType
 
 | typing_app f f_ty args T :
-    Σ ;; Γ |- f : f_ty ->
+    Σ ;; Γ ⊢ f : f_ty ->
     (*is_TApp f = false ->*)
     args <> [] ->
     All_spine (@typing) Σ Γ f_ty args T ->
-    Σ ;; Γ |- TApp f args : T
+    Σ ;; Γ ⊢ TApp f args : T
 
 | typing_evar ev entry :
     (*typing_context Σ Γ ->*)
     Σ ev = Some entry ->
-    Σ ;; Γ |- TEvar ev : wk entry.(evar_type)
+    Σ ;; Γ ⊢ TEvar ev : wk entry.(evar_type)
 
 | typing_conv_type t A B :
-    Σ ;; Γ |- t : A ->
-    Σ |- A ≡ B ->
-    Σ ;; Γ |- B : TType ->
-    Σ ;; Γ |- t : B
+    Σ ;; Γ ⊢ t : A ->
+    Σ ⊢ A ≡ B ->
+    Σ ;; Γ ⊢ B : TType ->
+    Σ ;; Γ ⊢ t : B
 
-where "Σ ;; Γ |- t : T" := (typing Σ Γ t T)
-  (*and "'typing_context' Σ Γ" := (All_context (fun _ Γ' t => Σ ;; Γ' |- t : TType) Γ)*).
+where "Σ ;; Γ ⊢ t : T" := (typing Σ Γ t T)
+  (*and "'typing_context' Σ Γ" := (All_context (fun _ Γ' t => Σ ;; Γ' ⊢ t : TType) Γ)*).
 
 Set Elimination Schemes.
 
 Derive Signature for typing.
 
-(** [typing_ren Σ Γ ρ Δ] means that the renaming [ρ] maps well-typed terms
+(** [Σ ;; Γ ⊢ᵣ ρ : Δ] means that the renaming [ρ] maps well-typed terms
     in context [Γ] to well-typed terms in context [Δ]. *)
-Definition typing_ren {s s'} Σ (Γ : context ∅ s) (ρ : ren s s') (Δ : context ∅ s') :=
-  forall i, Σ ;; Δ |- TVar (rapply ρ i) : rename ρ (lookup_context i Γ).
+Definition typing_ren {s s'} (Σ : evar_map) (Γ : context ∅ s) (ρ : ren s s') (Δ : context ∅ s') :=
+  forall i, rename ρ (lookup_context i Γ) = lookup_context (rapply ρ i) Δ.
 
-(** [typing_subst Σ Γ σ Δ] means that the substitution [σ] maps well-typed
+Notation "Σ ;; Γ ⊢ᵣ ρ : Δ" := (typing_ren Σ Γ ρ Δ)
+  (at level 50, Γ at next level, ρ at next level, Δ at next level).
+
+(** [Σ ;; Γ ⊢ₛ σ : Δ] means that the substitution [σ] maps well-typed
     terms in context [Γ] to well-typed terms in context [Δ]. *)
 Definition typing_subst {s s'} Σ (Γ : context ∅ s) (σ : subst s s') (Δ : context ∅ s') :=
-  forall i, Σ ;; Δ |- sapply σ i : substitute σ (lookup_context i Γ).
+  forall i, Σ ;; Δ ⊢ sapply σ i : substitute σ (lookup_context i Γ).
+
+Notation "Σ ;; Γ ⊢ₛ σ : Δ" := (typing_subst Σ Γ σ Δ)
+  (at level 50, Γ at next level, σ at next level, Δ at next level).
 
 (***********************************************************************)
 (** * Induction principle for [typing]. *)
@@ -123,28 +129,28 @@ Lemma typing_ind
   (Htype : forall s Σ Γ, P s Σ Γ TType TType)
   (Hvar : forall s Σ Γ i ty, lookup_context i Γ = ty -> P s Σ Γ (TVar i) ty)
   (Hlam : forall s Σ Γ x ty body body_ty,
-    Σ ;; Γ |- ty : TType -> P s Σ Γ ty TType ->
-    Σ ;; CCons Γ x ty |- body : body_ty -> P (s ▷ x) Σ (CCons Γ x ty) body body_ty ->
+    Σ ;; Γ ⊢ ty : TType -> P s Σ Γ ty TType ->
+    Σ ;; CCons Γ x ty ⊢ body : body_ty -> P (s ▷ x) Σ (CCons Γ x ty) body body_ty ->
     P s Σ Γ (TLam x ty body) (TProd x ty body_ty))
   (Hprod : forall s Σ Γ x a b,
-    Σ ;; Γ |- a : TType -> P s Σ Γ a TType ->
-    Σ ;; CCons Γ x a |- b : TType -> P (s ▷ x) Σ (CCons Γ x a) b TType ->
+    Σ ;; Γ ⊢ a : TType -> P s Σ Γ a TType ->
+    Σ ;; CCons Γ x a ⊢ b : TType -> P (s ▷ x) Σ (CCons Γ x a) b TType ->
     P s Σ Γ (TProd x a b) TType)
   (Happ : forall s Σ Γ f f_ty args T,
-    Σ ;; Γ |- f : f_ty -> P s Σ Γ f f_ty ->
+    Σ ;; Γ ⊢ f : f_ty -> P s Σ Γ f f_ty ->
     (*is_TApp f = false ->*)
     args <> [] ->
-    All_spine (fun s Σ Γ t T => Σ ;; Γ |- t : T /\ P s Σ Γ t T) Σ Γ f_ty args T ->
+    All_spine (fun s Σ Γ t T => Σ ;; Γ ⊢ t : T /\ P s Σ Γ t T) Σ Γ f_ty args T ->
     P s Σ Γ (TApp f args) T)
   (Hevar : forall s Σ Γ ev entry,
     Σ ev = Some entry ->
     P s Σ Γ (TEvar ev) (wk entry.(evar_type)))
   (Hconv_type : forall s Σ Γ t A B,
-    Σ ;; Γ |- t : A -> P s Σ Γ t A ->
-    Σ |- A ≡ B ->
-    Σ ;; Γ |- B : TType -> P s Σ Γ B TType ->
+    Σ ;; Γ ⊢ t : A -> P s Σ Γ t A ->
+    Σ ⊢ A ≡ B ->
+    Σ ;; Γ ⊢ B : TType -> P s Σ Γ B TType ->
     P s Σ Γ t B) :
-  forall s Σ Γ t T, Σ ;; Γ |- t : T -> P s Σ Γ t T.
+  forall s Σ Γ t T, Σ ;; Γ ⊢ t : T -> P s Σ Γ t T.
 Proof.
 fix IH 6. intros s Σ Γ t T H. depelim H.
 - apply Htype.
@@ -166,63 +172,51 @@ Qed.
 (***********************************************************************)
 
 Lemma typing_rid {s} Σ (Γ : context ∅ s) :
-  typing_ren Σ Γ rid Γ.
-Proof. intros i. simpl_subst. constructor. reflexivity. Qed.
+  Σ ;; Γ ⊢ᵣ rid : Γ.
+Proof. intros i. simpl_subst. reflexivity. Qed.
 
 Lemma typing_rshift {s x} Σ (Γ : context ∅ s) ty :
   typing_ren Σ Γ rshift (CCons Γ x ty).
 Proof.
-intros i. simpl_subst. constructor. simp lookup_context.
-unfold wk. cbn. now simpl_subst.
+intros i. simpl_subst. simp lookup_context. simpl_subst. reflexivity.
 Qed.
 
 Lemma typing_rcons {s s' x} Σ (Γ : context ∅ s) (Δ : context ∅ s') i ρ ty :
-  Σ ;; Δ |- TVar i : rename ρ ty ->
-  typing_ren Σ Γ ρ Δ ->
-  typing_ren Σ (CCons Γ x ty) (rcons x i ρ) Δ.
+  rename ρ ty = lookup_context i Δ ->
+  Σ ;; Γ ⊢ᵣ ρ : Δ ->
+  Σ ;; CCons Γ x ty ⊢ᵣ rcons x i ρ : Δ.
 Proof.
-intros H1 H2 j. depelim j ; simpl_subst ; simp lookup_context.
-- unfold wk. cbn. simpl_subst. assumption.
-- unfold wk. cbn. simpl_subst. apply H2.
+intros H1 H2 j. depelim j ; simpl_subst ; simp lookup_context ; simpl_subst.
+- assumption.
+- apply H2.
 Qed.
 
-(*Lemma rename_lookup_context {s s'} Σ Γ Δ (ρ : ren s s') i :
-  typing_ren Σ Γ ρ Δ ->
-  rename ρ (lookup_context i Γ) = lookup_context (rapply ρ i) Δ.
-Proof.
-intros H. specialize (H i).*)
-
 Lemma typing_rcomp {s s' s''} Σ Γ Δ E (ρ1 : ren s s') (ρ2 : ren s' s'') :
-  typing_ren Σ Γ ρ1 Δ ->
-  typing_ren Σ Δ ρ2 E ->
-  typing_ren Σ Γ (rcomp ρ1 ρ2) E.
+  Σ ;; Γ ⊢ᵣ ρ1 : Δ ->
+  Σ ;; Δ ⊢ᵣ ρ2 : E ->
+  Σ ;; Γ ⊢ᵣ rcomp ρ1 ρ2 : E.
 Proof.
-intros H1 H2 i. rewrite <-rename_rename, rapply_rcomp.
-specialize (H2 (rapply ρ1 i)).
-Admitted.
-(*Lemma typing_rename_rshift {s x} Σ Γ (t : term s) T xty :
-  Σ ;; Γ |- t : T ->
-  Σ ;; (CCons Γ x xty) |- rename rshift t : rename rshift T.
-Proof. Admitted.*)
+intros H1 H2 i. rewrite <-rename_rename. rewrite H1, H2. now simpl_subst.
+Qed.
 
 Lemma typing_rup {s s' x} Σ Γ Δ (ρ : ren s s') ty :
-  typing_ren Σ Γ ρ Δ ->
-  typing_ren Σ (CCons Γ x ty) (rup x ρ) (CCons Δ x (rename ρ ty)).
+  Σ ;; Γ ⊢ᵣ ρ : Δ ->
+  Σ ;; CCons Γ x ty ⊢ᵣ rup x ρ : CCons Δ x (rename ρ ty).
 Proof.
 intros H. unfold rup. apply typing_rcons.
-- constructor. simp lookup_context. unfold wk. cbn. now simpl_subst.
-- eapply typing_rcomp ; [|eapply typing_rshift]. assumption.
+- simp lookup_context. now simpl_subst.
+- eapply typing_rcomp ; eauto. apply typing_rshift.
 Qed.
 
 (** Compatibility of typing with renamings *)
 Lemma typing_rename {s s'} Σ Γ Δ (ρ : ren s s') t T :
-  Σ ;; Γ |- t : T ->
-  typing_ren Σ Γ ρ Δ ->
-  Σ ;; Δ |- rename ρ t : rename ρ T.
+  Σ ;; Γ ⊢ t : T ->
+  Σ ;; Γ ⊢ᵣ ρ : Δ ->
+  Σ ;; Δ ⊢ rename ρ t : rename ρ T.
 Proof.
 intros Ht Hρ. induction Ht in s', ρ, Δ, Hρ |- * ; simpl_subst.
 - apply typing_type.
-- rewrite <-H. apply Hρ.
+- rewrite <-H, Hρ. now constructor.
 - apply typing_lam ; auto using typing_rup.
 - apply typing_prod ; auto using typing_rup.
 - eapply typing_app.
@@ -234,28 +228,26 @@ intros Ht Hρ. induction Ht in s', ρ, Δ, Hρ |- * ; simpl_subst.
       apply All_spine_cons with (x := x) (a := rename ρ a) (b := rename (rup x ρ) b).
       --simpl_subst in H'. now apply H'.
       --rewrite H0. now simpl_subst.
-      --assert ((rename (rup x ρ) b)[x := rename ρ arg] = rename ρ (b[x := arg])) as ->.
-        { simpl_subst. f_equal. subst_ext i. depelim i ; now simpl_subst. }
-        apply IHAll_spine ; assumption.
+      --simpl_subst. simpl_subst in IHAll_spine. now apply IHAll_spine.
 - now apply typing_evar.
 - apply typing_conv_type with (A := rename ρ A) ; auto. now rewrite H.
 Qed.
 
 Lemma typing_sid {s} Σ (Γ : context ∅ s) :
-  typing_subst Σ Γ sid Γ.
+  Σ ;; Γ ⊢ₛ sid : Γ.
 Proof. intros i. simpl_subst. constructor. reflexivity. Qed.
 
 Lemma typing_sshift {s x} Σ (Γ : context ∅ s) ty :
-  typing_subst Σ Γ sshift (CCons Γ x ty).
+  Σ ;; Γ ⊢ₛ sshift : CCons Γ x ty.
 Proof.
 intros i. simpl_subst. constructor. simp lookup_context.
 unfold wk. cbn. simpl_subst. rewrite <-substitute_sren. reflexivity.
 Qed.
 
 Lemma typing_scons {s s' x} Σ (Γ : context ∅ s) (Δ : context ∅ s') t σ ty :
-  Σ ;; Δ |- t : substitute σ ty ->
-  typing_subst Σ Γ σ Δ ->
-  typing_subst Σ (CCons Γ x ty) (scons x t σ) Δ.
+  Σ ;; Δ ⊢ t : substitute σ ty ->
+  Σ ;; Γ ⊢ₛ σ : Δ ->
+  Σ ;; CCons Γ x ty ⊢ₛ scons x t σ : Δ.
 Proof.
 intros H1 H2 i. depelim i ; simpl_subst ; simp lookup_context.
 - unfold wk. cbn. simpl_subst. assumption.
@@ -263,26 +255,17 @@ intros H1 H2 i. depelim i ; simpl_subst ; simp lookup_context.
 Qed.
 
 Lemma typing_srcomp {s s' s''} Σ Γ Δ E (σ : subst s s') (ρ : ren s' s'') :
-  typing_subst Σ Γ σ Δ ->
-  typing_ren Σ Δ ρ E ->
-  typing_subst Σ Γ (srcomp σ ρ) E.
+  Σ ;; Γ ⊢ₛ σ : Δ ->
+  Σ ;; Δ ⊢ᵣ ρ : E ->
+  Σ ;; Γ ⊢ₛ srcomp σ ρ : E.
 Proof.
 intros H1 H2 i. simpl_subst. rewrite <-rename_substitute.
 eapply typing_rename ; [|eassumption]. apply H1.
 Qed.
 
-Lemma typing_rscomp {s s' s''} Σ Γ Δ E (ρ : ren s s') (σ : subst s' s'') :
-  typing_ren Σ Γ ρ Δ ->
-  typing_subst Σ Δ σ E ->
-  typing_subst Σ Γ (rscomp ρ σ) E.
-Proof.
-intros H1 H2 i. simpl_subst. rewrite <-substitute_rename.
-specialize (H2 (rapply ρ i)).
-Admitted.
-
 Lemma typing_sup {s s' x} Σ Γ Δ (σ : subst s s') ty :
-  typing_subst Σ Γ σ Δ ->
-  typing_subst Σ (CCons Γ x ty) (sup x σ) (CCons Δ x (substitute σ ty)).
+  Σ ;; Γ ⊢ₛ σ : Δ ->
+  Σ ;; CCons Γ x ty ⊢ₛ sup x σ : CCons Δ x (substitute σ ty).
 Proof.
 intros H. unfold sup. apply typing_scons.
 - constructor. simp lookup_context. unfold wk. cbn. simpl_subst. reflexivity.
@@ -290,9 +273,9 @@ intros H. unfold sup. apply typing_scons.
 Qed.
 
 Lemma typing_substitute {s s'} Σ Γ Δ (σ : subst s s') t T :
-  Σ ;; Γ |- t : T ->
-  typing_subst Σ Γ σ Δ ->
-  Σ ;; Δ |- substitute σ t : substitute σ T.
+  Σ ;; Γ ⊢ t : T ->
+  Σ ;; Γ ⊢ₛ σ : Δ ->
+  Σ ;; Δ ⊢ substitute σ t : substitute σ T.
 Proof.
 intros Ht Hσ. induction Ht in s', σ, Δ, Hσ |- * ; simpl_subst.
 - constructor.
@@ -305,27 +288,48 @@ intros Ht Hσ. induction Ht in s', σ, Δ, Hσ |- * ; simpl_subst.
     apply All_spine_cons with (x := x) (a := substitute σ a) (b := substitute (sup x σ) b).
     * simpl_subst in H. now apply H.
     * rewrite H0. simpl_subst. reflexivity.
-    * assert ((substitute (sup x σ) b)[x := substitute σ arg] = substitute σ (b[x := arg])) as ->.
-      { simpl_subst. f_equal. }
+    * simpl_subst. simpl_subst in IHAll_spine. now apply IHAll_spine.
+- econstructor ; eauto.
+- eapply typing_conv_type ; eauto. now rewrite H.
+Qed.
+
+Lemma typing_rscomp {s s' s''} Σ Γ Δ E (ρ : ren s s') (σ : subst s' s'') :
+  Σ ;; Γ ⊢ᵣ ρ : Δ ->
+  Σ ;; Δ ⊢ₛ σ : E ->
+  Σ ;; Γ ⊢ₛ rscomp ρ σ : E.
+Proof.
+intros H1 H2 i. rewrite <-substitute_rename.
+assert (sapply (rscomp ρ σ) i = substitute σ (TVar (rapply ρ i))) as -> by now simpl_subst.
+eapply typing_substitute ; eauto. rewrite H1. now constructor.
+Qed.
+
+Lemma typing_scomp {s s' s''} Σ Γ Δ E (σ1 : subst s s') (σ2 : subst s' s'') :
+  Σ ;; Γ ⊢ₛ σ1 : Δ ->
+  Σ ;; Δ ⊢ₛ σ2 : E ->
+  Σ ;; Γ ⊢ₛ scomp σ1 σ2 : E.
+Proof.
+intros H1 H2 i. simpl_subst. rewrite <-substitute_substitute.
+eapply typing_substitute ; eauto.
+Qed.
 
 (** Next define typing on evar-maps... *)
 
 
 Lemma typing_type_ok {s} Σ Γ (t T : term s) :
-  Σ ;; Γ |- t : T ->
-  Σ ;; Γ |- T : TType.
+  Σ ;; Γ ⊢ t : T ->
+  Σ ;; Γ ⊢ T : TType.
 Proof. Admitted.
 
 (** Reducing a term doesn't change its type. *)
 Lemma typing_red {s} Σ Γ (t u T : term s) :
-  Σ ;; Γ |- t : T ->
-  Σ |- t ~> u ->
-  Σ ;; Γ |- u : T.
+  Σ ;; Γ ⊢ t : T ->
+  Σ ⊢ t ~> u ->
+  Σ ;; Γ ⊢ u : T.
 Proof. Admitted.
 
 (** Changing a term to a convertible one doesn't change its type. *)
 Lemma typing_conv {s} Σ Γ (t u T : term s) :
-  Σ ;; Γ |- t : T ->
-  Σ |- t ≡ u ->
-  Σ ;; Γ |- u : T.
+  Σ ;; Γ ⊢ t : T ->
+  Σ ⊢ t ≡ u ->
+  Σ ;; Γ ⊢ u : T.
 Proof. Admitted.
